examples/sampler/p4ast.v
@@ -2452,12 +2452,7 @@ Definition SwitchIngressParser := DeclParser NoInfo
                                {| stags := NoInfo; str := "apply" |})
                           (TypFunction
                            (MkFunctionType nil
-                                [(MkParameter false Directionless
-                                      (TypExtern
-                                       {| stags := NoInfo;
-                                          str := "packet_in" |}) None
-                                      {| stags := NoInfo; str := "pkt" |});
-                                 (MkParameter false Out
+                                [(MkParameter false Out
                                       (TypHeader
                                        [( {| stags := NoInfo;
                                              str := "resubmit_flag" |},
@@ -2481,14 +2476,6 @@ Definition SwitchIngressParser := DeclParser NoInfo
                                          str := "ig_intr_md" |})] FunParser
                                 TypVoid)) Directionless) nil
                      [(Some
-                       (MkExpression NoInfo
-                            (ExpName
-                             (BareName {| stags := NoInfo; str := "pkt" |})
-                             (LInstance ["pkt"]))
-                            (TypTypeName
-                             {| stags := NoInfo; str := "packet_in" |})
-                            Directionless));
-                      (Some
                        (MkExpression NoInfo
                             (ExpName
                              (BareName
